sf/Assignment09_04.v
@@ -17,7 +17,14 @@ Example hoare_asgn_example4 :
   {{fun st => True}} (X ::= (ANum 1);; Y ::= (ANum 2)) 
   {{fun st => st X = 1 /\ st Y = 2}}.
 Proof.
-  exact FILL_IN_HERE.
+  eapply hoare_seq.
+    apply hoare_asgn.
+    eapply hoare_consequence.
+      apply hoare_asgn.
+      intros st H. assert (((fun st : state => st X = 1) [X |-> ANum 1]) st). reflexivity. apply H0.
+      intros st H. unfold assn_sub. simpl. unfold update. split.
+        destruct (eq_id_dec Y X). inversion e. apply H.
+        destruct (eq_id_dec Y Y). reflexivity. unfold not in n. apply ex_falso_quodlibet. apply n. reflexivity.
 Qed.
 
 (*-- Check --*)
